feat: nary `generalize` tactic
This commit also fixes a bug when using multiple targets with the
`induction` and `cases` tactics.

src/Lean/Meta/Tactic/Generalize.lean
@@ -5,24 +5,64 @@ Authors: Leonardo de Moura
 -/
 import Lean.Meta.KAbstract
 import Lean.Meta.Tactic.Util
+import Lean.Meta.Tactic.Intro
 
 namespace Lean.Meta
 
-def generalize (mvarId : MVarId) (e : Expr) (x : Name) (failIfNotInTarget : Bool := true) : MetaM MVarId :=
+/-- The `generalize` tactic takes arguments of the form `h : e = x` -/
+structure GeneralizeArg where
+  expr   : Expr
+  xName? : Option Name := none
+  hName? : Option Name := none
+  deriving Inhabited
+
+partial def generalize (mvarId : MVarId) (args : Array GeneralizeArg) : MetaM (Array FVarId × MVarId) :=
   withMVarContext mvarId do
     checkNotAssigned mvarId `generalize
     let tag ← getMVarTag mvarId
-    let target ← getMVarType mvarId
-    let target ← instantiateMVars target
-    let targetAbst ← kabstract target e
-    if failIfNotInTarget && !targetAbst.hasLooseBVars then
-      throwTacticEx `generalize mvarId "failed to find expression in the target"
-    let eType ← inferType e
-    let targetNew := Lean.mkForall x BinderInfo.default eType targetAbst
+    let target ← instantiateMVars (← getMVarType mvarId)
+    let rec go (i : Nat) : MetaM Expr := do
+      if i < args.size then
+        let arg := args[i]
+        let e ← instantiateMVars arg.expr
+        let eType ← instantiateMVars (← inferType e)
+        let type ← go (i+1)
+        let xName ← if let some xName := arg.xName? then pure xName else mkFreshUserName `x
+        return Lean.mkForall xName BinderInfo.default eType (← kabstract type e)
+      else
+        return target
+    let targetNew ← go 0
     unless (← isTypeCorrect targetNew) do
-      throwTacticEx `generalize mvarId "result is not type correct"
-    let mvarNew ← mkFreshExprSyntheticOpaqueMVar targetNew tag
-    assignExprMVar mvarId (mkApp mvarNew e)
-    pure mvarNew.mvarId!
+      throwTacticEx `generalize mvarId m!"result is not type correct{indentExpr targetNew}"
+    let es := args.map (·.expr)
+    if !args.any fun arg => arg.hName?.isSome then
+      let mvarNew ← mkFreshExprSyntheticOpaqueMVar targetNew tag
+      assignExprMVar mvarId (mkAppN mvarNew es)
+      introNP mvarNew.mvarId! args.size
+    else
+      let (rfls, targetNew) ← forallBoundedTelescope targetNew args.size fun xs type => do
+        let rec go' (i : Nat) : MetaM (List Expr × Expr) := do
+          if i < xs.size then
+            let arg := args[i]
+            if let some hName := arg.hName? then
+              let xType ← inferType xs[i]
+              let e ← instantiateMVars arg.expr
+              let eType ← instantiateMVars (← inferType e)
+              let (hType, r) ←
+                if (← isDefEq xType eType) then
+                  pure (← mkEq e xs[i], ← mkEqRefl e)
+                else
+                  pure (← mkHEq e xs[i], ← mkHEqRefl e)
+              let (rs, type) ← go' (i+1)
+              return (r :: rs, mkForall hName BinderInfo.default hType type)
+            else
+              go' (i+1)
+          else
+            return ([], type)
+        let (rfls, type) ← go' 0
+        return (rfls, ← mkForallFVars xs type)
+      let mvarNew ← mkFreshExprSyntheticOpaqueMVar targetNew tag
+      assignExprMVar mvarId (mkAppN (mkAppN mvarNew es) rfls.toArray)
+      introNP mvarNew.mvarId! (args.size + rfls.length)
 
 end Lean.Meta
