tests/lean/run/generalizeMany.lean
@@ -1,0 +1,13 @@
+def Fin.succ (v : Fin n) : Fin n.succ :=
+  match v with
+  | ⟨v, h⟩ => ⟨v+1, Nat.succ_lt_succ h⟩
+
+set_option pp.analyze false
+
+example (p : (n : Nat) → Fin n → Prop)
+        (n : Nat)
+        (v : Fin n)
+        : p n.succ v.succ := by
+  generalize h₁ : n.succ = n', h₂ : v.succ = v'
+  traceState
+  admit
