tests/lean/run/multiTargetCasesInductionIssue.lean
@@ -1,0 +1,47 @@
+def Vec (α : Type u) (n : Nat) : Type u := { a : List α // a.length = n }
+def Vec.nil : Vec α 0 := ⟨[], rfl⟩
+def Vec.cons (a : α) (as : Vec α n) : Vec α (n+1) := ⟨a :: as.val, by simp [as.property]⟩
+
+set_option pp.analyze false
+
+def Vec.casesOn
+     (motive : (n : Nat) → Vec α n → Sort v)
+     (n  : Nat)
+     (as : Vec α n)
+     (nil : motive 0 Vec.nil)
+     (cons : (n : Nat) → (a : α) → (as : Vec α n) → (ih : motive n as) → motive (n+1) (Vec.cons a as))
+     : motive n as :=
+  let rec go (n : Nat) (as : List α) (h : as.length = n) : motive n ⟨as, h⟩ :=
+    match n, as, h with
+    | 0,   [],    _ => nil
+    | n+1, a::as, h =>
+      have : as.length = n := by injection h; assumption
+      have ih : motive n ⟨as, this⟩ := go n as this
+      cons n a ⟨as, this⟩ ih
+  match as with
+  | ⟨as, h⟩ => go n as h
+
+example (n : Nat) (a : α) (as : Vec α n) : Vec.cons a (Vec.cons a as) = Vec.cons a (Vec.cons a as) := by
+  induction n+2, Vec.cons a (Vec.cons a as) using Vec.casesOn
+  case nil => constructor
+  case cons n a as ih =>
+    traceState
+    constructor
+
+#print "-----"
+
+example (n : Nat) (a : α) (as : Vec α n) : Vec.cons a (Vec.cons a as) = Vec.cons a (Vec.cons a as) := by
+  cases n+2, Vec.cons a (Vec.cons a as) using Vec.casesOn
+  case nil => constructor
+  case cons n a as ih =>
+    traceState
+    constructor
+
+#print "-----"
+
+example (n : Nat) (a : α) (as : Vec α n) : Vec.cons a (Vec.cons a as) = Vec.cons a (Vec.cons a as) := by
+  cases h₁ : n+2, h₂ : Vec.cons a (Vec.cons a as) using Vec.casesOn
+  case nil => constructor
+  case cons n' a' as' ih =>
+    traceState
+    constructor
